Main.lean
@@ -1,44 +1,34 @@
 import DqratLean
 
--- ─── Proof processor ───────────────────────────────────────────────────────
-
--- def processProof (st : CheckState) (content : String) : ProofResult :=
---   match (checkActions (parseProofActions content)).run st with
---   | .error e _ => .failed 0 #[e] #[] none
---   | .ok r _    => r
-
 def main : List String → IO UInt32
   | [formulaFile, proofFile] => do
-    let formula ← IO.FS.readFile formulaFile
-    let proof   ← IO.FS.readFile proofFile
-    match (parseDQDIMACS formula).run {} with
-    | .error (.failed _ es _ _) _ =>
-      for e in es do
+      let formulaContent ← IO.FS.readFile formulaFile
+      let proofContent   ← IO.FS.readFile proofFile
+      match parseDQDIMACS formulaContent with
+      | .error e =>
         IO.eprintln s!"c parse error: {e}"
-      return 1
-    | .error (.verified _) _ =>
-      -- Formula UNSAT by UP during parsing
-      IO.println "c formula found unsat during reading in"
-      IO.println "s VERIFIED"
-      return 0
-    | .ok _ st =>
-      IO.println s!"c formula read successfully"
-      let proof := parseProofActions proof
-      match (checkActions proof).run st with
-      | .error (.verified line) _ =>
-        IO.println s!"c line {line}: unit propagation derived conflict, proof valid"
+        return 1
+      | .ok none =>
+        -- Formula UNSAT by UP during parsing
+        IO.println "c formula found unsat during reading in"
         IO.println "s VERIFIED"
-      | .error (.failed line rules _info blocker) _ =>
-        let rulesStr := rules.foldl (· ++ ", " ++ ·) "" |>.drop 2
-        IO.println s!"c line {line}: lemma checked for: {rulesStr}"
-        if let some _ := blocker then
-          IO.println "c (blocker clause found)"
-        IO.println "c the check has failed. The proof is invalid"
-        IO.println "s FAILED"
-      | .ok _ _ =>
-        IO.println "c lemmas are correct, but there is no conflict at the end"
-        IO.println "s UNKNOWN"
-      return 0
+        return 0
+      | .ok (some st) =>
+        IO.println s!"c formula read successfully"
+        let result := processProof st proofContent
+        match result with
+        | .Verified line =>
+          IO.println s!"c line {line}: unit propagation derived conflict, proof valid"
+        | .Failed line rules _info blocker =>
+          let rulesStr := rules.foldl (· ++ ", " ++ ·) "" |>.drop 2
+          IO.println s!"c line {line}: lemma checked for: {rulesStr}"
+          if let some _ := blocker then
+            IO.println "c (blocker clause found)"
+          IO.println "c the check has failed. The proof is invalid"
+        | .Unknown =>
+          IO.println "c lemmas are correct, but there is no conflict at the end"
+        IO.println (formatResult result)
+        return 0
   | _ => do
       IO.println "Usage: dqrat-lean <formula.dqdimacs> <proof.dqrat>"
       return 1
